

TABLE 1 The Truth Table for the Negation of a Proposition.

p	$\neg p$
T	F
F	T

TABLE 2 The Truth Table for the Conjunction of Two Propositions.

p	q	$p \wedge q$
T	T	T
T	F	F
F	T	F
F	F	F

TABLE 3 The Truth Table for the Disjunction of Two Propositions.

p	q	$p \vee q$
T	T	T
T	F	T
F	T	T
F	F	F

TABLE 4 The Truth Table for the Exclusive Or of Two Propositions.

p	q	$p \oplus q$
T	T	F
T	F	T
F	T	T
F	F	F

TABLE 5 The Truth Table for the Conditional Statement $p \rightarrow q$.

p	q	$p \rightarrow q$
T	T	T
T	F	F
F	T	T
F	F	T

TABLE 6 The Truth Table for the Biconditional $p \leftrightarrow q$.

p	q	$p \leftrightarrow q$
T	T	T
T	F	F
F	T	F
F	F	T

TABLE 8 Precedence of Logical Operators.

Operator	Precedence
\neg	1
\wedge	2
\vee	3
\rightarrow	4
\leftrightarrow	5

TABLE 2 De Morgan's Laws.

$$\neg(p \wedge q) \equiv \neg p \vee \neg q$$

$$\neg(p \vee q) \equiv \neg p \wedge \neg q$$

Soal:
Pernyataan:
"Jika n^2 habis dibagi 3, maka n habis dibagi 9."

Counterexample Proof:

- Ambil $n = 3$
- $n^2 = 9 \rightarrow$ habis dibagi 3 ☒
- Tapi $n = 3 \rightarrow$ tidak habis dibagi 9 ☒
- Jadi pernyataan salah, dan $n = 3$ adalah counterexample ☒

Equivalence	Name
$p \wedge \mathbf{T} \equiv p$ $p \vee \mathbf{F} \equiv p$	Identity laws
$p \vee \mathbf{T} \equiv \mathbf{T}$ $p \wedge \mathbf{F} \equiv \mathbf{F}$	Domination laws
$p \vee p \equiv p$ $p \wedge p \equiv p$	Idempotent laws
$\neg(\neg p) \equiv p$	Double negation law
$p \vee q \equiv q \vee p$ $p \wedge q \equiv q \wedge p$	Commutative laws
$(p \vee q) \vee r \equiv p \vee (q \vee r)$ $(p \wedge q) \wedge r \equiv p \wedge (q \wedge r)$	Associative laws
$p \vee (q \wedge r) \equiv (p \vee q) \wedge (p \vee r)$ $p \wedge (q \vee r) \equiv (p \wedge q) \vee (p \wedge r)$	Distributive laws
$\neg(p \wedge q) \equiv \neg p \vee \neg q$ $\neg(p \vee q) \equiv \neg p \wedge \neg q$	De Morgan's laws
$p \vee (p \wedge q) \equiv p$ $p \wedge (p \vee q) \equiv p$	Absorption laws
$p \vee \neg p \equiv \mathbf{T}$ $p \wedge \neg p \equiv \mathbf{F}$	Negation laws

Equivalence	Name
$p \rightarrow q \equiv \neg p \vee q$	
$p \rightarrow q \equiv \neg q \rightarrow \neg p$	
$p \vee q \equiv \neg p \rightarrow q$	
$p \wedge q \equiv \neg(p \rightarrow \neg q)$	
$\neg(p \rightarrow q) \equiv p \wedge \neg q$	
$(p \rightarrow q) \wedge (p \rightarrow r) \equiv p \rightarrow (q \wedge r)$	
$(p \rightarrow r) \wedge (q \rightarrow r) \equiv (p \vee q) \rightarrow r$	
$(p \rightarrow q) \vee (p \rightarrow r) \equiv p \rightarrow (q \vee r)$	
$(p \rightarrow r) \vee (q \rightarrow r) \equiv (p \wedge q) \rightarrow r$	

Equivalence	Name
$p \leftrightarrow q \equiv (p \rightarrow q) \wedge (q \rightarrow p)$	
$p \leftrightarrow q \equiv \neg p \leftrightarrow \neg q$	
$p \leftrightarrow q \equiv (p \wedge q) \vee (\neg p \wedge \neg q)$	
$\neg(p \leftrightarrow q) \equiv p \leftrightarrow \neg q$	

Definition
Another way to create a proposition from propositional function

In English words
all, some, many, none, and few

Types

- Universal quantifier \rightarrow For all values... $\forall x P(x)$
- Existential quantifier \rightarrow For some values in... $\exists x P(x)$
- Unique quantifier \rightarrow For one values in... $\exists! x P(x)$

Negation of Quantifiers
Every student in your class has taken a course in calculus

$\forall x P(x)$

Negation \rightarrow It is not the case that every student in your class has taken a course in calculus

Equivalent to \rightarrow There is a student in your class who has not taken a course in calculus

$\exists x \neg P(x)$

Conclude as $\neg \forall x P(x) \equiv \exists x \neg P(x)$

De Morgan's Law

$$\neg(p \wedge q) \equiv \neg p \vee \neg q$$

$$\neg(p \vee q) \equiv \neg p \wedge \neg q$$

p	q	$\neg p$	$\neg q$	$p \vee q$	$\neg(p \vee q)$	$(\neg p) \wedge (\neg q)$
0	0	1	1	0	1	1
0	1	1	0	1	0	0
1	0	0	1	1	0	0
1	1	0	0	1	0	0

Proof by Contraposition

Making use of the fact that the conditional statement $p \rightarrow q$ is equivalent to its contrapositive, $\neg q \rightarrow \neg p$

e.g. in $p \rightarrow q$,

We get the contrapositive $\neg q \rightarrow \neg p$

Take $\neg q$ as premise

we show that $\neg p$ must follow

Logical operators

- NOT (negation)
- AND (conjunction)
- Inclusive OR (disjunction)
- EXclusive OR (XOR)
- Conditional statement (implication)
- Biconditional (iff)

Symbol \neg

Symbol \wedge

Symbol \vee

Symbol \oplus

Symbol \rightarrow

Symbol \leftrightarrow

Buktikan:
"Ada tepat satu bilangan bulat x sehingga $2x + 3 = 11$."

Penyelesaian (Unique Proof):

1. Existence:

- Cari x yang memenuhi: $2x + 3 = 11 \implies 2x = 8 \implies x = 4$
- Jadi ada $x = 4$ yang memenuhi ☒

2. Uniqueness:

- Misal ada y lain yang juga memenuhi: $2y + 3 = 11 \implies 2y = 8 \implies y = 4$
- Jadi $y = x = 4$
- Tidak mungkin ada bilangan lain yang memenuhi ☒

Kesimpulan: Ada tepat satu bilangan bulat $x = 4$ ☒

Proof of Equivalence

To prove a theorem that is a biconditional statement $p \leftrightarrow q$ we show that $p \rightarrow q$ and $q \rightarrow p$ are both true.

Based on the tautology $(p \leftrightarrow q) \leftrightarrow (p \rightarrow q) \wedge (q \rightarrow p)$

Vacuous Proof

$p \rightarrow q$ is true if p is false

p	q	$p \rightarrow q$
0	0	1
0	1	1
1	0	0
1	1	1

Trivial Proof

$p \rightarrow q$ is true if q is true

p	q	$p \rightarrow q$
0	0	1
0	1	1
1	0	0
1	1	1

Proofs

if $n > 1$ then $n^2 > n$, for $n = 0$

$p : 0 > 1$ (FALSE)

$q : 0^2 > 0$ (FALSE)

hence $p \rightarrow q$ TRUE

domain: all integers

if $a \geq b$ then $a^0 \geq b^0$ a, b are positive integers and $n = 0$

$p : a \geq b$

$q : a^0 \geq b^0$ (TRUE)

hence, the theorem is true

domain: positive integers

TABLE 1 Rules of Inference.

Rule of Inference	Tautology	Name
$\frac{p \quad p \rightarrow q}{\therefore q}$	$(p \wedge (p \rightarrow q)) \rightarrow q$	Modus ponens
$\frac{\neg q \quad p \rightarrow q}{\therefore \neg p}$	$(\neg q \wedge (p \rightarrow q)) \rightarrow \neg p$	Modus tollens
$\frac{p \rightarrow q \quad q \rightarrow r}{\therefore p \rightarrow r}$	$((p \rightarrow q) \wedge (q \rightarrow r)) \rightarrow (p \rightarrow r)$	Hypothetical syllogism
$\frac{p \vee q \quad \neg p}{\therefore q}$	$((p \vee q) \wedge \neg p) \rightarrow q$	Disjunctive syllogism
$\frac{p}{\therefore p \vee q}$	$p \rightarrow (p \vee q)$	Addition
$\frac{p \wedge q}{\therefore p}$	$(p \wedge q) \rightarrow p$	Simplification
$\frac{p \quad q}{\therefore p \wedge q}$	$((p) \wedge (q)) \rightarrow (p \wedge q)$	Conjunction
$\frac{p \vee q \quad \neg p \vee r}{\therefore q \vee r}$	$((p \vee q) \wedge (\neg p \vee r)) \rightarrow (q \vee r)$	Resolution

STEP 1	
Kalimat	Simbol
It rains	R
It is foggy	F
The sailing race will be held	S
The lifesaving demonstration will go on	L
The trophy will be awarded	T

STEP 2	
Kalimat	Simbol
"If it does not rain or if it is not foggy, then the sailing race will be held and the lifesaving demonstration will go on"	$(\neg R \vee \neg F) \rightarrow (S \wedge L)$
"If the sailing race is held, then the trophy will be awarded"	$S \rightarrow T$
"The trophy was not awarded"	$\neg T$
"It rained"	R

STEP 3		
No	Langkah	Alasan
1	$\neg T$	Premis
2	$S \rightarrow T$	Premis
3	$\neg S$	Modus Tollens (1) dan (2)
4	$(\neg R \vee \neg F) \rightarrow (S \wedge L)$	Premis
5	$\neg(S \wedge L) \rightarrow \neg(\neg R \vee \neg F)$	Contrapositive
6	$\neg S \vee \neg L \rightarrow (R \wedge F)$	De Morgan's Law
7	$\neg S \vee \neg L$	Addition Rule dari $\neg S$ (3)
8	$(R \wedge F)$	Modus Ponens (6) dan (7)
9	R	Simplification

STEP 1	
Kalimat	Simbol
x is a student in this class	$C(x)$
x has read the book	$B(x)$
x passed the first exam	$P(x)$

STEP 2	
Kalimat	Simbol
"A student in this class has not read the book"	$\exists x(C(x) \wedge \neg B(x))$
"Everyone in this class passed the first exam"	$\forall x(C(x) \rightarrow P(x))$
"Someone who passed the first exam has not read the book"	$\exists x(P(x) \wedge \neg B(x))$

STEP 3	
No	Langkah
1	$\exists x(C(x) \wedge \neg B(x))$
2	$C(a) \wedge \neg B(a)$
3	$C(a)$
4	$\forall x(C(x) \rightarrow P(x))$
5	$C(a) \rightarrow P(a)$
6	$P(a)$
7	$\neg B(a)$
8	$P(a) \wedge \neg B(a)$
9	$\exists x(P(x) \wedge \neg B(x))$

STEP 3	
Langkah	Alasan
$\exists x(C(x) \wedge \neg B(x))$	Premis
$C(a) \wedge \neg B(a)$	Existential instantiation dari (1)
$C(a)$	Simplification dari (2)
$\forall x(C(x) \rightarrow P(x))$	Premis
$C(a) \rightarrow P(a)$	Universal instantiation dari (4)
$P(a)$	Modus Ponens dengan (5) dengan (3)
$\neg B(a)$	Simplification of $C(a) \wedge \neg B(a)$ / (2)
$P(a) \wedge \neg B(a)$	Conjunction between (6) and (7)
$\exists x(P(x) \wedge \neg B(x))$	Existential Generalization

Contoh:

Jika $3n + 2$ genap, maka n genap.

Bukti kontradiksi:

- Asumsikan $3n + 2$ genap (P) dan n ganjil ($\neg Q$)
- Dari n ganjil, kita dapat $3n + 2$ ganjil. Tapi itu **berlawanan** dengan $3n + 2$ genap.
- Kontradiksi \rightarrow asumsi salah \rightarrow maka n genap.

Soal:

Buktikan:

"Jika x ganjil, maka x^2 ganjil."

Penyelesaian (Forward Reasoning):

- Diketahui: x ganjil $\rightarrow x = 2k + 1$
- Hitung x^2 :

$$x^2 = (2k + 1)^2 = 4k^2 + 4k + 1 = 2(2k^2 + 2k) + 1$$

- Karena $x^2 = 2(\text{bilangan bulat}) + 1$, maka x^2 ganjil \checkmark

Penalaran maju ini langsung dari fakta ke kesimpulan tanpa mundur dari tujuan.

Buktikan:

"Jika $x + 1$ ganjil, maka x genap."

Penyelesaian (Backward Reasoning):

- Tujuan: Buktikan $x \text{ genap} \rightarrow x = 2k$
- Diketahui: $x + 1$ ganjil $\rightarrow x + 1 = 2m + 1$
- Maka $x = (2m + 1) - 1 = 2m \rightarrow$ genap \checkmark

Rule of Inference	Name
$\frac{\forall x P(x)}{\therefore P(c)}$	Universal instantiation
$\frac{P(c) \text{ for an arbitrary } c}{\therefore \forall x P(x)}$	Universal generalization
$\frac{\exists x P(x)}{\therefore P(c) \text{ for some element } c}$	Existential instantiation
$\frac{P(c) \text{ for some element } c}{\therefore \exists x P(x)}$	Existential generalization

Soal:

Buktikan bahwa untuk setiap bilangan bulat n dengan $1 \leq n \leq 4$, $n^2 \leq 16$.

Penyelesaian (exhaustive proof):

Periksa semua nilai $n = 1, 2, 3, 4$:

- $n = 1: 1^2 = 1 \leq 16 \checkmark$
- $n = 2: 2^2 = 4 \leq 16 \checkmark$
- $n = 3: 3^2 = 9 \leq 16 \checkmark$
- $n = 4: 4^2 = 16 \leq 16 \checkmark$

"Jika n adalah bilangan bulat, maka $n^2 + n$ adalah genap."

Penyelesaian (Proof by Cases):

- Kasus 1: n genap, misal $n = 2k$
 - $n^2 + n = (2k)^2 + 2k = 4k^2 + 2k = 2(2k^2 + k) \checkmark$ genap
- Kasus 2: n ganjil, misal $n = 2k + 1$
 - $n^2 + n = (2k + 1)^2 + (2k + 1) = 4k^2 + 4k + 1 + 2k + 1 = 4k^2 + 6k + 2 = 2(2k^2 + 3k + 1) \checkmark$ genap

Karena kedua kasus menunjukkan hasil genap, pernyataan benar untuk semua bilangan bulat n .

Contoh Soal 3 (lebih abstrak)

Soal:

Buktikan:

"Untuk setiap bilangan bulat positif n , ada bilangan bulat positif m sehingga $m > n$."

Penyelesaian (Construction Proof):

- Cara konstruksi: ambil $m = n + 1$
- Jelas $m > n$ dan m positif \checkmark

Kita menunjukkan secara langsung cara membuat m yang memenuhi, jadi bukti selesai.

Soal:

Buktikan:

"Ada bilangan prima yang lebih besar dari 1000."

Penyelesaian (Non-Construction Proof):

- Kita tahu bilangan prima tak terbatas (Teorema Euclid).
- Maka pasti ada bilangan prima yang lebih besar dari 1000. \checkmark
- Kita tidak menulis bilangannya, cukup argumen eksistensi.

Teks soal. Use a proof by contraposition to show: if $x + y \geq 2$ (real x, y) then $x \geq 1$ or $y \geq 1$.

$\neg(x \geq 1 \vee y \geq 1) \rightarrow \neg(x + y \geq 2)$

$\neg(x \geq 1) \wedge \neg(y \geq 1) \rightarrow \neg(x + y \geq 2)$

$x < 1 \wedge y < 1 \rightarrow x + y < 2$ **benar**